cogent/isa/Cogent.thy
@@ -398,7 +398,23 @@ lemma type_wellformed_pretty_intros:
 
 definition type_wellformed_all_pretty :: "kind env \<Rightarrow> type list \<Rightarrow> bool" ("_ \<turnstile>* _ wellformed" [30,20] 60) where
   "K \<turnstile>* ts wellformed \<equiv> list_all (type_wellformed (length K)) ts"
-declare type_wellformed_all_pretty_def[simp]
+
+lemma type_wellformed_all_Cons[simp]:
+  "K \<turnstile>* t # ts wellformed = (K \<turnstile> t wellformed \<and> K \<turnstile>* ts wellformed)"
+  by (simp add: type_wellformed_all_pretty_def)
+
+lemma type_wellformed_all_Nil[simp,intro!]:
+  "K \<turnstile>* [] wellformed"
+  by (simp add: type_wellformed_all_pretty_def)
+
+lemma type_wellformed_all_length:
+  "K \<turnstile>* ts wellformed = (\<forall>i<length ts. K \<turnstile> ts ! i wellformed)"
+  by (simp add: type_wellformed_all_pretty_def list_all_length)
+
+lemma type_wellformed_all_iff:
+  "K \<turnstile>* ts wellformed = (\<forall>x\<in>set ts. K \<turnstile> x wellformed)"
+  by (simp add: type_wellformed_all_pretty_def list_all_iff)
+
 
 definition proc_ctx_wellformed :: "('f \<Rightarrow> poly_type) \<Rightarrow> bool" where
   "proc_ctx_wellformed \<Xi> = (\<forall> f. let (K, \<tau>i, \<tau>o) = \<Xi> f in K \<turnstile> TFun \<tau>i \<tau>o wellformed)"
@@ -424,6 +440,11 @@ definition kinding :: "kind env \<Rightarrow> type \<Rightarrow> kind \<Rightarr
 lemma kindingI:
   "K \<turnstile> t wellformed \<Longrightarrow> k \<subseteq> kinding_fn K t \<Longrightarrow> K \<turnstile> t :\<kappa> k"
   by (simp add: kinding_def)
+
+lemma kinding_kinding_allI:
+  "K \<turnstile> t wellformed \<Longrightarrow> K \<turnstile> t :\<kappa> (kinding_fn K t)"
+  by (simp add: kinding_def)
+
 
 definition kinding_all :: "kind env \<Rightarrow> type list \<Rightarrow> kind \<Rightarrow> bool" ("_ \<turnstile>* _ :\<kappa> _" [30,0,30] 60) where
   "K \<turnstile>* ts :\<kappa> k \<equiv> (\<forall>t\<in>set ts. K \<turnstile> t wellformed) \<and> k \<subseteq> (\<Inter>t\<in>set ts. kinding_fn K t)"
@@ -643,7 +664,6 @@ lemmas weakening_conv_all_nth = list_all2_conv_all_nth[where P="weakening_comp K
 definition is_consumed :: "kind env \<Rightarrow> ctx \<Rightarrow> bool" ("_ \<turnstile> _ consumed" [30,20] 60 ) where
   "K \<turnstile> \<Gamma> consumed \<equiv> K \<turnstile> \<Gamma> \<leadsto>w empty (length \<Gamma>)"
 
-declare is_consumed_def [simp]
 
 section {* Built-in types *}
 
@@ -975,6 +995,7 @@ fun type_repr :: "type \<Rightarrow> repr" where
 | "type_repr (TUnit)              = RUnit"
 
 
+
 section {* Wellformed lemmas *}
 
 lemma wellformed_record_wellformed_elem:
@@ -1039,7 +1060,7 @@ lemma kinding_iff_wellformed:
     "(\<exists>k. K \<turnstile>* ts :\<kappa> k) \<longleftrightarrow> K \<turnstile>* ts wellformed"
     "(\<exists>k. K \<turnstile>* tvs :\<kappa>v k) \<longleftrightarrow> K \<turnstile>* map (fst \<circ> snd) tvs wellformed"
     "(\<exists>k. K \<turnstile>* trs :\<kappa>r k) \<longleftrightarrow> K \<turnstile>* map (fst \<circ> snd) trs wellformed"
-  by (auto simp add: kinding_defs list_all_iff)
+  by (force simp add: list_all_iff kinding_defs type_wellformed_all_pretty_def)+
 
 lemma kinding_to_wellformedD:
   shows
@@ -1047,7 +1068,7 @@ lemma kinding_to_wellformedD:
     "K \<turnstile>* ts :\<kappa> k \<Longrightarrow> K \<turnstile>* ts wellformed"
     "K \<turnstile>* tvs :\<kappa>v k \<Longrightarrow> K \<turnstile>* map (fst \<circ> snd) tvs wellformed"
     "K \<turnstile>* trs :\<kappa>r k \<Longrightarrow> K \<turnstile>* map (fst \<circ> snd) trs wellformed"
-  by (auto simp add: kinding_defs list_all_iff)
+  by (force simp add: list_all_iff kinding_defs type_wellformed_all_pretty_def)+
 
 lemma list_all2_kinding_wellformedD:
   "list_all2 (kinding K) ts K' \<Longrightarrow> list_all (type_wellformed (length K)) ts \<and> length ts = length K'"
@@ -1163,7 +1184,8 @@ lemma variant_tagged_list_update_wellformedI:
     "K \<turnstile>* map (fst \<circ> snd) ts wellformed"
   shows "K \<turnstile> TSum (tagged_list_update n (t, b) ts) wellformed"
   using assms
-  by (induct ts arbitrary: n t b; fastforce simp add: list_all_iff)
+  by (induct ts arbitrary: n t b)
+     (fastforce simp add: type_wellformed_all_pretty_def comp_def list.pred_map)+
 
 lemma variant_tagged_list_update_kinding:
   assumes "n \<in> fst ` set ts"
@@ -1328,7 +1350,8 @@ and   "K \<turnstile>* ts wellformed \<Longrightarrow> k \<subseteq> {D, S} \<Lo
 and   "K \<turnstile>* map (fst \<circ> snd) xs wellformed \<Longrightarrow> k \<subseteq> {D, S} \<Longrightarrow> K \<turnstile>* map (\<lambda>(n,t,b). (n, bang t, b)) xs :\<kappa>v k"
 and   "K \<turnstile>* map (fst \<circ> snd) fs wellformed \<Longrightarrow> k \<subseteq> {D, S} \<Longrightarrow> K \<turnstile>* map (\<lambda>(n,t,b). (n, bang t, b)) fs :\<kappa>r k"
   using bang_wellformed bang_kinding_fn
-  by (fastforce simp add: kinding_defs INT_subset_iff list_all_iff simp del: insert_subset
+  by (fastforce simp add: kinding_defs INT_subset_iff type_wellformed_all_iff
+      simp del: insert_subset
       split: variant_state.split record_state.split)+
 
 section {* Subtyping lemmas *}
@@ -1861,7 +1884,8 @@ lemma instantiate_ctx_consumed [simplified]:
 assumes "K \<turnstile> \<Gamma> consumed"
 and     "list_all2 (kinding K') \<delta> K"
 shows   "K' \<turnstile> instantiate_ctx \<delta> \<Gamma> consumed"
-using assms by (auto intro: instantiate_ctx_weaken [where \<Gamma>' = "empty (length \<Gamma>)", simplified])
+  using assms
+  by (auto intro: instantiate_ctx_weaken[where \<Gamma>' = "empty (length \<Gamma>)", simplified] simp add: is_consumed_def)
 
 lemma map_option_instantiate_split_comp:
 assumes "K \<turnstile> c \<leadsto> c1 \<parallel> c2"
@@ -2147,13 +2171,18 @@ lemma weakening_nth:
 assumes weak: "K \<turnstile> \<Gamma> \<leadsto>w \<Gamma>'"
 and           "i < length \<Gamma>"
 shows         "weakening_comp K (\<Gamma>!i) (\<Gamma>'!i)"
-using assms by (auto simp add: weakening_def dest: list_all2_nthD)
+  using assms by (auto simp add: weakening_def dest: list_all2_nthD)
 
 lemma weakening_refl:
   "K \<turnstile> xs \<leadsto>w xs"
   by (clarsimp simp add: weakening_conv_all_nth weakening_comp.simps)
 
+lemma consumed_replicate_None[simp,intro!]:
+  "K \<turnstile> replicate n None consumed"
+  by (induct n) (simp add: is_consumed_def Cogent.empty_def weakening_refl)+
 
+
+section {* wellformed and kinding lemmas *}
 
 lemma typing_to_wellformed:
 shows "\<Xi>, K, \<Gamma> \<turnstile>  e  : t  \<Longrightarrow> K \<turnstile>  t  wellformed"
@@ -2168,7 +2197,7 @@ next case typing_fun then show ?case
 next case typing_esac then show ?case
     by (fastforce dest: filter_member2  simp add: kinding_simps kinding_variant_set list_all_iff)
 next case typing_struct then show ?case
-    by (simp add: list_all_zip_iff_list_all2 list_all2_conv_all_nth list_all_length)
+    by (simp add: list_all_zip_iff_list_all2 list_all2_conv_all_nth type_wellformed_all_length list_all_length)
 next case typing_member then show ?case
     by (fastforce simp add: kinding_defs INT_subset_iff list_all_iff dest: nth_mem split: prod.splits record_state.splits)
 next case typing_put then show ?case
@@ -2203,7 +2232,7 @@ lemma wellformed_bang_type_repr[simp]:
     and "[] \<turnstile>* ts wellformed \<Longrightarrow> (map (type_repr \<circ> bang) ts) = map (type_repr) ts "
     and "[] \<turnstile>* map (fst \<circ> snd) xs wellformed \<Longrightarrow> (map (type_repr \<circ>  bang \<circ> fst \<circ> snd) xs) = map (type_repr \<circ> fst \<circ> snd) xs"
     and "[] \<turnstile>* map (fst \<circ> snd) fs wellformed \<Longrightarrow> (map (type_repr \<circ>  bang \<circ> fst \<circ> snd) fs) = map (type_repr \<circ> fst \<circ> snd) fs"
-  by (clarsimp simp add: wellformed_imp_bang_type_repr map_eq_iff_nth_eq list_all_length simp del: map_eq_conv)+
+  by (clarsimp simp add: wellformed_imp_bang_type_repr map_eq_iff_nth_eq type_wellformed_all_length simp del: map_eq_conv)+
 
 lemma bang_type_repr[simp]:
   shows "[] \<turnstile> t :\<kappa> k \<Longrightarrow> (type_repr (bang t) = type_repr t)"
